\documentclass[12pt]{article}

\title{Group Homework 6}
\author{G2 - Robert Krency, Austin Pringle, Anthony Stepich}
\date{\today}

\usepackage{amsmath}
\usepackage{graphicx}
\usepackage{tabularx}
\usepackage{multicol}
\usepackage{enumitem}

% Geometry 
\usepackage{geometry}
\geometry{letterpaper, left=15mm, top=20mm, right=15mm, bottom=20mm}

% Add vertical spacing to tables
\renewcommand{\arraystretch}{2}

% Macros
\newcommand{\definition}[1]{\underline{\textbf{#1}}}

% Begin Document
\begin{document}

\maketitle

\begin{enumerate}

    %1
    \item $f(X, Y, Z) = Y + X'Y'Z'$ \\
    \begin{tabular}{r l l}
        = & $Y + (X + Y + Z)'$ & \\
        = & $((Y')(X + Y + Z))' $ & \\
        = & $(Y'X + Y'Y + Y'Z)'$ & \\
        = & $(Y'X + Y'Z)'$ & \\
        = & $(Y'X)'(Y'Z)'$ & \\
        = & $(Y + X')(Y + Z')$ & \\
        = & $YY + YZ' + X'Y + X'Z'$ & \\
        = & $Y(1 + Z' + X') + X'Z'$ & \\
        = & $Y + X'Z'$ & \\
    \end{tabular}
    
    \pagebreak
    
    %2
    \item $f(X, Y, Z) = (X + Y)(X + Z)(Z + Y)$ \\
    \begin{tabular}{r l}
        = & $(XX + XZ + XY + YZ)(Z + Y)$ \\
        = & $XZ + XY + XZY + YZ$ \\ 
        = & $XZ + XY(1 + Z) + YZ$ \\
        = & $XZ + XY + YZ$ \\ 
    \end{tabular}

    \vspace{20mm}

    %3
    \item $f(X, Y, Z) = X'Y' + X'Y + YZ' + XZ'$ \\
    \begin{tabular}{r l l}
        = & $X'(Y' + Y) + YZ' + XZ'$ & \\
        = & $X' + YZ' + XZ'$ & \\
        = & $((X)(XZ')'(YZ')')'$ &\\
        = & $((X)(X' + Z)(Y' + Z))'$ &\\
        = & $((X)(X'Y' + X'Z + Y'Z + ZZ))'$ & \\
        = & $(XX'Y' + XX'Z + XY'Z + XZ)'$ & \\
        = & $(XZ(Y' + 1))'$ & \\
        = & $(XZ)'$ & \\
        = & $X' + Z'$ & \\ 
    \end{tabular}
    
    \pagebreak
    
    % 4
    \item $f(W, X, Y, Z) = YW + X'YZ' + XZ'W + XYZ + X'ZW$ \\
    \begin{tabular}{r l l}
        = & $YW + Y(X'Z' + XZ) + W(XZ' + X'Z)$ & \\
        = & $YW + Y(X'Z + XZ')' + W(XZ' + X'Z)$ & \\
        = & $Y(X'Z + XZ')' + W(XZ' + X'Z)$ & Theorem 3 \\
        = & $X'YZ' + XZ'W + XYZ + X'ZW$ & \\
    \end{tabular}
    
    \pagebreak
    
    % 5
    \item $f(X, Y, Z) = (X + Z)(X + Y')(Y + Z)$ \\
    \begin{tabular}{r l l}
        = & $(X + XY' + ZX + ZY')(Y + Z)$ & \\
        = & $XY + XZ + XY'Y + XY'Z + ZXY + ZXZ + ZY'Y + ZY'Z$ & \\
        = & $XY + XZ + XY'Z + XYZ + ZY'$ & \\
        = & $XY + XZ + XZ(Y' + Y) + ZY'$ & \\
        = & $XY + XZ + ZY'$ & \\
    \end{tabular}
    
    \vspace{20mm}
    
    % 6
    \item $f(W, X, Y, Z) = (W' + X')' (Y + Z)'$\\
    \begin{tabular}{r l l}
        = & $WX(Y+Z)'$ & \\
        = & $WX(Y'Z')$ & \\
        = & $WXY'Z'$ & \\
    \end{tabular}
    
    \pagebreak
    
    %7
    \item $f(X, Y, Z) = (X + Y)(X' + Y)(X + Y')(X' + Y')$ \\
    \begin{tabular}{r l l}
        = & $(XX' + XY + X'Y + YY)(XX' + XY' + X'Y' + Y'Y')$ & \\
        = & $(XY + X'Y + Y)(XY' + X'Y' + Y')$ & \\
        = & $Y(X + X' + 1)Y'(X + X' + 1)$ & \\
        = & $YY'$ & \\
        = & $0$ & \\
    \end{tabular}
    
    \pagebreak
    
    %8
    \item $f(A, B, C, D) = AB + A'C + B'CD$ \\
    \begin{tabular}{r l l}
        = & $AB(C + C')(D + D') + A'(B + B')C(D + D') + (A + A')B'CD$ & \\
        = & $ABCD + ABC'D + ABCD + ABC'D' + A'BCD + A'B'CD + A'BCD' + A'B'CD' + AB'CD + A'B'CD$ & \\
        = & $BCD + B'CD + ABC'D + ABC'D' + BCD' + A'B'CD' + A'B'CD$ & \\
        = & $BD + ABC' + BC + A'B'C$ & \\
        = & $BD + ABC' + BC(A + A') + A'B'C$ & \\
        = & $BC + ABC' + ABC + A'BC + A'B'C$ & \\
        = & $BD + AB + A'C$ & \\
    \end{tabular}
    
    \pagebreak
    
    %9
    \item $f(A, B, C, D) = AB + A'C + B'D + CD$ \\
    \begin{tabular}{r l l}
        = & $ $ & \\
        = & $ $ & \\
        = & $ $ & \\
        = & $ $ & \\
        = & $ $ & \\
    \end{tabular}
    
    \pagebreak
    
    %10
    \item $f(X, Y, Z) = (X'(XY'Z')')Z$ \\
    \begin{tabular}{r l l}
        = & $Z(X'(X' + Y + Z))'$ & \\
        = & $Z(X'X' + X'Y + X'Z)'$ & \\
        = & $Z(X'(1 + Y + Z))'$ & \\
        = & $Z(X')'$ & \\
        = & $ZX$ & \\
    \end{tabular}

\end{enumerate}

\end{document}